Finished the proof of FlatAsmgen

x86/FlatAsmgen.v
@@ -801,11 +801,31 @@ Proof.
   apply Forall_dec. intros. apply zlt.
 Defined.
 
+Definition main_exists main (defs: list (ident * option (AST.globdef Asm.fundef unit))) :=
+  Exists (fun '(id, def) => 
+            main = id 
+            /\ match def with
+              | None => False
+              | Some _ => True
+              end) defs.
+
+Definition main_exists_dec main defs : {main_exists main defs } + {~ main_exists main defs}.
+Proof.
+  apply Exists_dec. intros. destruct x.
+  generalize (ident_eq main i). intros.
+  destruct o; inv H.
+  - left. auto.
+  - right. inversion 1. auto.
+  - right. inversion 1. auto.
+  - right. inversion 1. auto.
+Qed.
+
 Record wf_prog (p:Asm.program) : Prop :=
   {
     wf_prog_not_empty: defs_not_empty (map snd (AST.prog_defs p));
     wf_prog_norepet_defs: list_norepet (map fst (AST.prog_defs p));
     wf_prog_norepet_labels: defs_no_duplicated_labels (AST.prog_defs p);
+    wf_prog_main_exists: main_exists (AST.prog_main p) (AST.prog_defs p);
   }.
 
 Definition check_wellformedness p : { wf_prog p } + { ~ wf_prog p }.
@@ -813,7 +833,9 @@ Proof.
   destruct (defs_not_empty_dec (map snd (AST.prog_defs p))).
   destruct (list_norepet_dec ident_eq (map fst (AST.prog_defs p))).
   destruct (Forall_dec _ globdef_no_duplicated_labels_dec (map snd (AST.prog_defs p))).
+  destruct (main_exists_dec (AST.prog_main p) (AST.prog_defs p)).
   left; constructor; auto.
+  right. inversion 1. apply n. apply wf_prog_main_exists0.
   right; inversion 1. apply n. apply wf_prog_norepet_labels0.
   right; inversion 1. apply n. apply wf_prog_norepet_defs0.
   right; inversion 1. apply n. apply wf_prog_not_empty0.
